Matrices/carrier.v
@@ -1,0 +1,26 @@
+Require Export ZArithRing.
+Require Export ZArith.
+
+Module Type Carrier.
+Parameter A : Set.
+Parameter Aopp : A -> A.
+Parameters (Aplus Aminus Amult: A -> A -> A).
+Parameters (A0 : A) (A1 : A).
+
+Axiom A_ring : ring_theory A0 A1 Aplus Amult Aminus Aopp (eq(A:=A)).
+
+End Carrier.
+
+Module Zc : Carrier.
+
+Definition A := Z.
+Definition Aopp := Zopp.
+Definition Aplus := Zplus.
+Definition Aminus := Zminus.
+Definition Amult := Zmult.
+Definition A0 := 0%Z.
+Definition A1 := 1%Z.
+
+Definition A_ring := InitialRing.Zth.
+
+End Zc.
